working on hybrid parsing machinery with sid

RiscvDialect/LLVMRiscv/LLVMAndRiscV.lean
@@ -37,10 +37,10 @@ abbrev LLVMPlusRiscV : Dialect where
 
 namespace LLVMPlusRiscV.Op
 
-def llvm (llvmOp : LLVM.Op) : LLVMPlusRiscV.Op :=
-  --((@id (Dialect.Op LLVMPlusRiscV) <|
-    LLVMRiscV.Op.llvm llvmOp
-    --))
+-- def llvm (llvmOp : LLVM.Op) : LLVMPlusRiscV.Op :=
+--   --((@id (Dialect.Op LLVMPlusRiscV) <|
+--     LLVMRiscV.Op.llvm llvmOp
+--     --))
 
 
 end LLVMPlusRiscV.Op
@@ -51,7 +51,7 @@ instance : TyDenote (Dialect.Ty LLVMPlusRiscV) where
     | .riscv riscvTy => TyDenote.toType riscvTy
 
 @[simp]
-instance : DialectSignature LLVMPlusRiscV where
+instance LLVMPlusRiscVSignature : DialectSignature LLVMPlusRiscV where
   signature
   | .llvm llvmOp => .llvm <$> DialectSignature.signature llvmOp
   | .riscv riscvOp => .riscv <$> DialectSignature.signature riscvOp
@@ -89,7 +89,7 @@ def extractriscvArgs : LLVMRiscV.Op → RISCV64.RV64.Op
 #check LLVMRiscV.Op.llvm _
 #check LLVMPlusRiscV.Op
 -- #check (LLVMPlusRiscV.Op).llvm
-#check (LLVMPlusRiscV.Op.llvm _  )
+-- #check (LLVMPlusRiscV.Op.llvm _  )
 
 #check ((@id (Dialect.Op LLVMPlusRiscV) <| LLVMRiscV.Op.llvm _))
 #check (Dialect.Op LLVMPlusRiscV)
@@ -104,7 +104,7 @@ example (d : Dialect) : d.Ty := by
 -- args : HVector toType (argumentTypes llvmOp : List LLVM.Ty)
 -- args[i] : toType (argumentTypes ...)[i]
 
-#check LLVMPlusRiscV.Op.llvm
+-- #check LLVMPlusRiscV.Op.llvm
 def llvmArgsFromHybrid : {tys : List LLVM.Ty} → HVector TyDenote.toType (tys.map LLVMRiscV.Ty.llvm) → HVector TyDenote.toType tys
   | [], .nil => .nil
   | _ :: _, .cons x xs => .cons x (llvmArgsFromHybrid xs)
@@ -134,6 +134,26 @@ def ctxtTransformToLLVM  (Γ : Ctxt LLVMPlusRiscV.Ty) :=
     | .riscv _  => .bitvec 999
   ) Γ
 
+#check Ctxt
+
+#check Ctxt.Hom
+
+
+-- def Ctxt.filterMap.aux (Γ : Ctxt Ty) (f : Ty → Option Ty') (iΓ : Nat) : Σ (Δ : Ctxt Ty'), Fin   :=
+--   match Γ with
+--   | [] => []
+--   | t :: ts =>
+--     match f t with
+--     | .none => Ctxt.filterMap.aux ts f
+--     | .some t' => t' :: Ctxt.filterMap.aux ts f
+
+-- def ctxtTransformToLLVM? (Γ : Ctxt LLVMPlusRiscV.Ty) : Ctxt LLVM.Ty :=
+--   Ctxt.filterMap.aux Γ (fun ty =>
+--     match ty with
+--     | .llvm ty => some ty
+--     | _ => none
+--   )
+
 def ctxtTransformToRiscV (Γ : Ctxt LLVMPlusRiscV.Ty) :=
   Ctxt.map  (fun ty  =>
     match ty with
@@ -141,28 +161,80 @@ def ctxtTransformToRiscV (Γ : Ctxt LLVMPlusRiscV.Ty) :=
     | _  => .bv -- unsure what to return here because want to signal in case transformation is not valid
   ) Γ
 
+/-- Projection of `outTy` commutes with `Signature.map`. -/
+@[simp]
+theorem outTy_map_signature_eq {s : Signature α} {f : α → β} :
+  Signature.outTy (f <$> s) = f s.outTy := rfl
 
-def transformExprLLVM (e : Expr (InstCombine.MetaLLVM 0) (ctxtTransformToLLVM Γ) eff ty) :=
-  match e with
-  | Expr.mk op1 ty_eq1 eff_le1 args1 regArgs1 =>
-      Expr.mk
-      (op := LLVMPlusRiscV.Op.llvm op1 )
-      (eff_le := eff_le1 )
-      (ty_eq := by rfl)
-      (args := _ )-- .cons e₁ <| .cons e₂ .nil)
-      (regArgs := HVector.nil)
-      -- LLVMPlusRiscV Γ eff (.llvm ty)
+-- @bollu says @salinhkuhn should work directly on lean-mlir, rather than using as a submodule,
+-- because the development is complex enough to constantly add new features into lena-mlir
+def _root_.HVector.foldlM {B : Type*} [Monad m] (f : ∀ (a : α), B → A a → m B) :
+    ∀ {l : List α}, (init : B) → (as : HVector A l) → m B
+  | [],   b, .nil       => return b
+  | t::_, b, .cons a as => do foldlM f (← f t b a) as
 
-def transformExprLLVMCasesArgs  (e : Expr (InstCombine.MetaLLVM 0) (ctxtTransformToLLVM Γ) eff ty) :=
-  match e with
-  | Expr.mk op1 ty_eq1 eff_le1 args regArgs1 =>
-      Expr.mk
-      (op := LLVMPlusRiscV.Op.llvm op1 )
-      (eff_le := eff_le1 )
-      (ty_eq := by rfl)
-      (args := _ )-- .cons e₁ <| .cons e₂ .nil)
-      (regArgs := HVector.nil)
-      -- LLVMPlusRiscV Γ eff (.llvm ty)
+/-- Simultaneous map on the type and value level of an HVector. -/
+def _root_.HVector.ubermap {A : α → Type} {B : β → Type}
+    {l : List α}
+    (F : α → β)
+    (f : {a : α} → (v : A a) → B (F a) )
+    (as : HVector A l) : (HVector B (F <$> l)) :=
+  match l, as with
+  | [], .nil => .nil
+  | _t :: _ts, .cons a as => HVector.cons (f a) (HVector.ubermap F f as)
+
+/--
+Simultaneous map on the type and value level of an HVector while performing monadic effects for value translation.
+-/
+def _root_.HVector.ubermapM [Monad m] {A : α → Type} {B : β → Type}
+    {l : List α}
+    {F : α → β}
+    (f : (a : α) → (v : A a) → m (B (F a)) )
+    (as : HVector A l) : m (HVector B (F <$> l)) :=
+  match l, as with
+  | [], .nil => return .nil
+  | t :: _ts, .cons a as => do return HVector.cons (← f t a) (← HVector.ubermapM f as)
+
+def transformExprLLVM (e : Expr (InstCombine.MetaLLVM 0) (ctxtTransformToLLVM Γ) eff ty) :
+  MLIR.AST.ReaderM (LLVMPlusRiscV) (Expr LLVMPlusRiscV Γ eff (.llvm ty)) :=
+    match e with
+    | Expr.mk op1 ty_eq1 eff_le1 args1 regArgs1 => do
+        -- args1 : HVector (Ctxt.Var (ctxtTransformToLLVM Γ)) (DialectSignature.sig op1)
+        let args' : HVector (Ctxt.Var Γ) (.llvm <$> DialectSignature.sig op1) ←
+          args1.ubermapM fun t v => do
+            match h : Γ.get? v.val with
+            | some ty' => do
+              match hty : ty' with
+              | .riscv _ =>
+                throw <| .generic s!"INTERNAL ERROR: This case is impossible, LLVM expression is pointing to RISCV variable."
+              | .llvm originalLLVMTy =>
+                if hty' : originalLLVMTy = t then
+                  return ⟨v.val, by rw [h, hty']⟩
+                else
+                  throw <|.generic s!"INTERNAL ERROR: This case is impossible, LLVM expression is pointing to an incorrect bitwidth LLVM argument."
+                  -- return ⟨v.val, by rw [h]⟩
+            | none =>
+              -- this is impossible, because ctxtTransformToLLVM is a `List.map`, which always maintains length.
+              -- sorry
+              throw <| .generic s!"INTERNAL ERROR: This case is impossible, as 'ctxtTransformToLLVM' is length-preserving."
+        return Expr.mk
+          (op := Op.llvm op1)
+          (eff_le := eff_le1)
+          (ty_eq := ty_eq1 ▸ rfl) -- @bollu: Discussion with Alex needed about cute-ism.
+          (args := args')-- .cons e₁ <| .cons e₂ .nil)
+          (regArgs := HVector.nil)
+        -- LLVMPlusRiscV Γ eff (.llvm ty)
+
+-- def transformExprLLVMCasesArgs  (e : Expr (InstCombine.MetaLLVM 0) (ctxtTransformToLLVM Γ) eff ty) :=
+--   match e with
+--   | Expr.mk op1 ty_eq1 eff_le1 args regArgs1 =>
+--       Expr.mk
+--       (op := LLVMPlusRiscV.Op.llvm op1 )
+--       (eff_le := eff_le1 )
+--       (ty_eq := by rfl)
+--       (args := _ )-- .cons e₁ <| .cons e₂ .nil)
+--       (regArgs := HVector.nil)
+--       -- LLVMPlusRiscV Γ eff (.llvm ty)
 /-
 
 def rem {Γ : Ctxt _} (e₁ e₂: Ctxt.Var Γ .bv) : Expr RV64 Γ .pure .bv  :=
@@ -176,22 +248,23 @@ def rem {Γ : Ctxt _} (e₁ e₂: Ctxt.Var Γ .bv) : Expr RV64 Γ .pure .bv  :=
 -/
 
 
-
-
 #check Expr.mk
 #check Ctxt.Var
 
-def transformExprRiscV (e : Expr (InstCombine.MetaLLVM 0) (ctxtTransformToLLVM Γ) eff ty) :  Expr LLVMPlusRiscV Γ eff (LLVMRiscV.Ty.llvm ty)  :=
-  sorry
+-- def transformExprRiscV (e : Expr (InstCombine.MetaLLVM 0) (ctxtTransformToLLVM Γ) eff ty) :  Expr LLVMPlusRiscV Γ eff (LLVMRiscV.Ty.llvm ty)  :=
+--   sorry
 
 def mkExpr (Γ : Ctxt _) (opStx : MLIR.AST.Op 0) :
   MLIR.AST.ReaderM (LLVMPlusRiscV) (Σ eff ty, Expr (LLVMPlusRiscV) Γ eff ty) := do
 
-  let llvmParse := InstcombineTransformDialect.mkExpr (ctxtTransformToLLVM  Γ) opStx (← read)
+  let llvmParse := InstcombineTransformDialect.mkExpr (ctxtTransformToLLVM  Γ) opStx (← read) -- reading state out of the monad.
   match llvmParse with
-    | .ok ⟨eff, ty, expr⟩ => -- returns llvm expression
-      return ⟨eff, (.llvm ty),  expr⟩
-      --llvmParse
+    | .ok ⟨eff, ty, expr⟩ => do -- returns llvm expression
+      let v ← transformExprLLVM expr
+      return ⟨eff, .llvm ty, v⟩
+
+      -- return ⟨eff, (.llvm ty),  .llvm expr⟩
+      -- llvmParse
        -- transform the expression back
     | .error (.unsupportedOp _) => do
      let ⟨eff, (ty) , expr⟩ ← RiscvMkExpr.mkExpr (ctxtTransformToRiscV Γ) opStx (← read)
