RiscvDialect/LLVMRiscv/InstructionRewrites.lean
@@ -5,7 +5,7 @@ open riscv.semantics
 open LLVM
 
 -- llvm.add
-def add_llvm : Com  llvm.riscv [.opt64, .opt64] .pure .opt64  := [_| {
+def add_llvm : Com  llvm.riscv [.bitvec, .bitvec] .pure .bitvec  := [_| {
     ^entry (%lhs: !i64, %rhs: !i64 ):
       %add = "llvm.add"(%lhs, %rhs) : (!i64, !i64) -> !i64
       "return" (%add) : (!i64) -> ()
@@ -22,7 +22,7 @@ def add_riscv := [_| {
       "return" (%addl) : (!i64) -> ()
   }]
 
-def llvm_add_lower_riscv : RiscVPeepholeRewriteRefine [Ty.opt64, Ty.opt64] :=
+def llvm_add_lower_riscv : RiscVPeepholeRewriteRefine [Ty.bitvec, Ty.bitvec] :=
   {lhs:= add_llvm , rhs:= add_riscv ,
    correct := by
     unfold add_llvm add_riscv
@@ -35,6 +35,302 @@ def llvm_add_lower_riscv : RiscVPeepholeRewriteRefine [Ty.opt64, Ty.opt64] :=
       ]
     rintro (_|_) (_|_) <;> simp [add?]
   }
+
+
+/- # AND -/
+def and_llvm : Com  llvm.riscv [.bitvec, .bitvec] .pure .bitvec  := [_| {
+    ^entry (%lhs: !i64, %rhs: !i64 ):
+      %add = "llvm.and"(%lhs, %rhs) : (!i64, !i64) -> !i64
+      "return" (%add) : (!i64) -> ()
+  }]
+def and_riscv := [_| {
+    ^entry (%lhs: !i64, %rhs: !i64 ):
+      %lhsr = "builtin.unrealized_conversion_cast.LLVMToriscv"(%lhs) : (!i64) -> !r64
+      %rhsr = "builtin.unrealized_conversion_cast.LLVMToriscv"(%rhs) : (!i64) -> !r64
+      %add = "riscv.and"(%lhsr, %rhsr) : (!r64, !r64) -> !r64
+      %addl = "builtin.unrealized_conversion_cast.riscvToLLVM" (%add) : (!r64) -> (!i64)
+      "return" (%addl) : (!i64) -> ()
+  }]
+
+def llvm_and_lower_riscv : RiscVPeepholeRewriteRefine [Ty.bitvec, Ty.bitvec] :=
+  {lhs:= and_llvm , rhs:= and_riscv ,
+   correct := by
+    unfold and_llvm and_riscv
+    simp_peephole
+    simp [riscv.semantics.builtin.unrealized_conversion_cast.riscvToLLVM,  riscv.semantics.builtin.unrealized_conversion_cast.LLVMToriscv, RTYPE_pure64_RISCV_SUB]
+    simp [LLVM.and, RTYPE_pure64_RISCV_AND]
+    rintro (_|_) (_|_) <;> simp [and?]; bv_decide
+  }
+
+
+/- # ASHR  -/
+
+def ashr_llvm : Com  llvm.riscv [.bitvec, .bitvec] .pure .bitvec  := [_| {
+    ^entry (%lhs: !i64, %rhs: !i64 ):
+      %add = "llvm.ashr"(%lhs, %rhs) : (!i64, !i64) -> !i64
+      "return" (%add) : (!i64) -> ()
+  }]
+#eval ashr_llvm
+-- riscv.add
+def sra_riscv := [_| {
+    ^entry (%lhs: !i64, %rhs: !i64 ):
+      %lhsr = "builtin.unrealized_conversion_cast.LLVMToriscv"(%lhs) : (!i64) -> !r64
+      %rhsr = "builtin.unrealized_conversion_cast.LLVMToriscv"(%rhs) : (!i64) -> !r64
+      %add = "riscv.sra"(%lhsr, %rhsr) : (!r64, !r64) -> !r64
+      %addl = "builtin.unrealized_conversion_cast.riscvToLLVM" (%add) : (!r64) -> (!i64)
+      "return" (%addl) : (!i64) -> ()
+  }]
+
+def llvm_ahr_lower_riscv : RiscVPeepholeRewriteRefine [Ty.bitvec, Ty.bitvec] :=
+  {lhs:= ashr_llvm , rhs:= sra_riscv ,
+   correct := by
+    unfold ashr_llvm sra_riscv
+    simp_peephole
+    simp [riscv.semantics.builtin.unrealized_conversion_cast.riscvToLLVM,  riscv.semantics.builtin.unrealized_conversion_cast.LLVMToriscv, RTYPE_pure64_RISCV_SRA]
+   --help
+    --rintro (_|_) (_|_) <;> simp [];
+  }
+/- # LSHR  -/
+
+
+
+/- # MUL  -/
+def mul_llvm : Com  llvm.riscv [.bitvec, .bitvec] .pure .bitvec  := [_| {
+    ^entry (%lhs: !i64, %rhs: !i64 ):
+      %add = "llvm.mul"(%lhs, %rhs) : (!i64, !i64) -> !i64
+      "return" (%add) : (!i64) -> ()
+  }]
+#eval mul_llvm
+-- riscv.add
+def mul_riscv := [_| {
+    ^entry (%lhs: !i64, %rhs: !i64 ):
+      %lhsr = "builtin.unrealized_conversion_cast.LLVMToriscv"(%lhs) : (!i64) -> !r64
+      %rhsr = "builtin.unrealized_conversion_cast.LLVMToriscv"(%rhs) : (!i64) -> !r64
+      %add = "riscv.mul"(%lhsr, %rhsr) : (!r64, !r64) -> !r64
+      %addl = "builtin.unrealized_conversion_cast.riscvToLLVM" (%add) : (!r64) -> (!i64)
+      "return" (%addl) : (!i64) -> ()
+  }]
+
+def llvm_mul_lower_riscv : RiscVPeepholeRewriteRefine [Ty.bitvec, Ty.bitvec] :=
+  {lhs:= mul_llvm , rhs:= mul_riscv ,
+   correct := by
+    unfold mul_llvm mul_riscv
+    simp_peephole
+    simp [riscv.semantics.builtin.unrealized_conversion_cast.riscvToLLVM,  riscv.semantics.builtin.unrealized_conversion_cast.LLVMToriscv, MUL_pure64_ftt]
+    rintro (_|_) (_|_) <;> simp [mul]
+    . simp [mul?] --HELP
+      bv_decide
+
+
+
+/-
+
+    simp [riscv.semantics.builtin.unrealized_conversion_cast.riscvToLLVM,
+      riscv.semantics.builtin.unrealized_conversion_cast.LLVMToriscv,
+      riscv.semantics.RTYPE_pure64_RISCV_ADD,
+      add, liftM, monadLift, MonadLift.monadLift,
+      BitVec.Refinement.some_some
+      ]
+      -/
+
+  }
+
+/- # NEG , not in llvm  -/
+
+
+/- # NOT , not in llvm   -/
+
+
+/- # OR   -/
+def or_llvm : Com  llvm.riscv [.bitvec, .bitvec] .pure .bitvec  := [_| {
+    ^entry (%lhs: !i64, %rhs: !i64 ):
+      %add = "llvm.or"(%lhs, %rhs) : (!i64, !i64) -> !i64
+      "return" (%add) : (!i64) -> ()
+  }]
+def or_riscv := [_| {
+    ^entry (%lhs: !i64, %rhs: !i64 ):
+      %lhsr = "builtin.unrealized_conversion_cast.LLVMToriscv"(%lhs) : (!i64) -> !r64
+      %rhsr = "builtin.unrealized_conversion_cast.LLVMToriscv"(%rhs) : (!i64) -> !r64
+      %add = "riscv.or"(%lhsr, %rhsr) : (!r64, !r64) -> !r64
+      %addl = "builtin.unrealized_conversion_cast.riscvToLLVM" (%add) : (!r64) -> (!i64)
+      "return" (%addl) : (!i64) -> ()
+  }]
+
+def llvm_or_lower_riscv : RiscVPeepholeRewriteRefine [Ty.bitvec, Ty.bitvec] :=
+  {lhs:= or_llvm , rhs:= or_riscv ,
+   correct := by
+    unfold or_llvm or_riscv
+    simp_peephole
+    simp [riscv.semantics.builtin.unrealized_conversion_cast.riscvToLLVM,  riscv.semantics.builtin.unrealized_conversion_cast.LLVMToriscv, RTYPE_pure64_RISCV_OR, DisjointFlag.mk]
+    rintro (_|_) (_|_) <;> simp
+
+   -- bv_decide
+  }
+
+/- # REM  -/
+
+
+/- # SDIV   -/
+
+/- # SHL   -/
+def sll_llvm : Com  llvm.riscv [.bitvec, .bitvec] .pure .bitvec  := [_| {
+    ^entry (%lhs: !i64, %rhs: !i64 ):
+      %add = "llvm.shl"(%lhs, %rhs) : (!i64, !i64) -> !i64
+      "return" (%add) : (!i64) -> ()
+  }]
+#eval sll_llvm
+
+-- riscv.add
+def sll_riscv := [_| {
+    ^entry (%lhs: !i64, %rhs: !i64 ):
+      %lhsr = "builtin.unrealized_conversion_cast.LLVMToriscv"(%lhs) : (!i64) -> !r64
+      %rhsr = "builtin.unrealized_conversion_cast.LLVMToriscv"(%rhs) : (!i64) -> !r64
+      %add = "riscv.sll"(%lhsr, %rhsr) : (!r64, !r64) -> !r64
+      %addl = "builtin.unrealized_conversion_cast.riscvToLLVM" (%add) : (!r64) -> (!i64)
+      "return" (%addl) : (!i64) -> ()
+  }]
+
+axiom X : Prop
+axiom Y : Prop
+axiom Z : Prop
+
+-- (a b : Nat) ()
+-- subtraction_self_inverse
+-- sub_add_eq
+-- sub_eq_zero
+-- sub_self_eq
+
+def llvm_sll_lower_riscv : RiscVPeepholeRewriteRefine [Ty.bitvec, Ty.bitvec] :=
+  {lhs:= sll_llvm , rhs:= sll_riscv ,
+   correct := by
+    unfold sll_llvm sll_riscv
+    simp_peephole
+    simp only [builtin.unrealized_conversion_cast.riscvToLLVM, RTYPE_pure64_RISCV_SLL,
+      builtin.unrealized_conversion_cast.LLVMToriscv, Nat.sub_zero, Nat.reduceAdd,
+      BitVec.extractLsb_toNat, Nat.shiftRight_zero, Nat.reducePow, BitVec.shiftLeft_eq]
+    simp only [shl, Bool.false_eq_true, BitVec.shiftLeft_eq', BitVec.sshiftRight_eq', ne_eq,
+      false_and, ↓reduceIte, BitVec.ushiftRight_eq', Option.bind_eq_bind]
+
+    rintro (_|v) (_|w) <;> simp only [shl?, Nat.cast_ofNat, BitVec.ofNat_eq_ofNat, ge_iff_le,
+      BitVec.shiftLeft_eq', Option.some_bind, Option.none_bind, Option.getD_none, Option.getD_some,
+      BitVec.zero_shiftLeft, BitVec.Refinement.none_left]
+    split
+    case isTrue h =>
+      simp [BitVec.Refinement]
+    case isFalse h =>
+      simp only [BitVec.Refinement.some_some]
+      have h₁ (n : Nat) (b : Nat) (premise : (b < n) ) :  (b % n) = b := by
+        exact Nat.mod_eq_of_lt premise
+      have shift_left_mod {n : Nat} (a : BitVec n) (b : Nat)(h : b < n) :
+        a <<< b = a <<< (b % n) := by
+        rw [h₁]
+        exact h
+      apply shift_left_mod
+      simp only [BitVec.le_def, BitVec.toNat_ofNat, Nat.reducePow, Nat.reduceMod, not_le] at h
+      exact h
+  }
+
+
+/- # SUB   -/
+def sub_llvm : Com  llvm.riscv [.bitvec, .bitvec] .pure .bitvec  := [_| {
+    ^entry (%lhs: !i64, %rhs: !i64 ):
+      %add = "llvm.sub"(%lhs, %rhs) : (!i64, !i64) -> !i64
+      "return" (%add) : (!i64) -> ()
+  }]
+#eval sub_llvm
+
+-- riscv.add
+def sub_riscv := [_| {
+    ^entry (%lhs: !i64, %rhs: !i64 ):
+      %lhsr = "builtin.unrealized_conversion_cast.LLVMToriscv"(%lhs) : (!i64) -> !r64
+      %rhsr = "builtin.unrealized_conversion_cast.LLVMToriscv"(%rhs) : (!i64) -> !r64
+      %add = "riscv.sub"(%lhsr, %rhsr) : (!r64, !r64) -> !r64
+      %addl = "builtin.unrealized_conversion_cast.riscvToLLVM" (%add) : (!r64) -> (!i64)
+      "return" (%addl) : (!i64) -> ()
+  }]
+
+def llvm_sub_lower_riscv : RiscVPeepholeRewriteRefine [Ty.bitvec, Ty.bitvec] :=
+  {lhs:= sub_llvm , rhs:= sub_riscv ,
+   correct := by
+    unfold sub_llvm sub_riscv
+    simp_peephole
+    simp [riscv.semantics.builtin.unrealized_conversion_cast.riscvToLLVM,  riscv.semantics.builtin.unrealized_conversion_cast.LLVMToriscv, RTYPE_pure64_RISCV_SUB]
+    simp [sub]
+    rintro (_|_) (_|_) <;> simp [sub?]
+  }
+
+
+/- # UDIV   -/
+
+/- # UREM   -/
+
+/- # XOR   -/
+def xor_llvm : Com  llvm.riscv [.bitvec, .bitvec] .pure .bitvec  := [_| {
+    ^entry (%lhs: !i64, %rhs: !i64 ):
+      %add = "llvm.xor"(%lhs, %rhs) : (!i64, !i64) -> !i64
+      "return" (%add) : (!i64) -> ()
+  }]
+#eval sub_llvm
+
+-- riscv.add
+def xor_riscv := [_| {
+    ^entry (%lhs: !i64, %rhs: !i64 ):
+      %lhsr = "builtin.unrealized_conversion_cast.LLVMToriscv"(%lhs) : (!i64) -> !r64
+      %rhsr = "builtin.unrealized_conversion_cast.LLVMToriscv"(%rhs) : (!i64) -> !r64
+      %add = "riscv.xor"(%lhsr, %rhsr) : (!r64, !r64) -> !r64
+      %addl = "builtin.unrealized_conversion_cast.riscvToLLVM" (%add) : (!r64) -> (!i64)
+      "return" (%addl) : (!i64) -> ()
+  }]
+
+def llvm_xor_lower_riscv : RiscVPeepholeRewriteRefine [Ty.bitvec, Ty.bitvec] :=
+  {lhs:= xor_llvm , rhs:= xor_riscv ,
+   correct := by
+    unfold xor_llvm xor_riscv
+    simp_peephole
+    simp [riscv.semantics.builtin.unrealized_conversion_cast.riscvToLLVM,  riscv.semantics.builtin.unrealized_conversion_cast.LLVMToriscv, RTYPE_pure64_RISCV_XOR]
+    rintro (_|_) (_|_) <;> simp [LLVM.xor]
+    simp [xor?]
+    bv_decide
+  }
+
+
+/-
+[riscv.semantics.builtin.unrealized_conversion_cast.riscvToLLVM,
+      riscv.semantics.builtin.unrealized_conversion_cast.LLVMToriscv,
+      riscv.semantics.RTYPE_pure64_RISCV_ADD,
+      add, liftM, monadLift, MonadLift.monadLift,
+      BitVec.Refinement.some_some
+      ]
+
+
+-/
+
+
+
+
+
+
+
+
+
+
+
+
+
+
+
+
+
+
+
+
+
+
+
+
+
+
+
 
 /--
 ## Testing the application of cast "folding" pass/rewrites.
@@ -49,6 +345,7 @@ def ex1_rewritePeepholeAtO1 :
 
 
 def add_cast_eq_add_elim_rewrite :
-  Com llvm.riscv (Ctxt.ofList [.opt64, .opt64]) .pure .opt64 := rewritePeepholeAt (RiscVPeepholeRewriteRefine.toPeepholeUNSOUND llvm_add_lower_riscv) 1  add_riscv
+  Com llvm.riscv (Ctxt.ofList [.bitvec, .bitvec]) .pure .bitvec := rewritePeepholeAt (RiscVPeepholeRewriteRefine.toPeepholeUNSOUND llvm_add_lower_riscv) 1  add_riscv
 -- if dont provide a proof it fails to apply/ display the rewrite.
+
 #eval add_cast_eq_add_elim_rewrite
